Multiple improvements
- Fixed the syntax of EReceive - remove_message was missing
- Simple concurrent equivalences - which have not that simple proofs
- => direction of the map-parallel map equivalence

src/Concurrent/Experimental/MapPmap.v
@@ -1,4 +1,4 @@
-From CoreErlang.Concurrent Require Import BarbedBisim.
+From CoreErlang.Concurrent Require Import BisimReductions.
 From CoreErlang.FrameStack Require Import SubstSemantics Examples.
 
 Import ListNotations.
@@ -17,16 +17,166 @@ Proof.
     apply IHstep_rt.
 Qed.
 
+(* Everything which falls under the n_other category can be lifted to
+   inter-process level *)
+Theorem process_local_to_node :
+  forall p p' l ι, p -⌈l⌉->* p' ->
+    Forall (fun a => a = τ \/ a = ε \/ a = ASelf ι) l ->
+    forall O eth Π,
+      (eth, ι ↦ p ∥ Π) -[map (fun a => (a, ι)) l]ₙ->*
+      (eth, ι ↦ p' ∥ Π) with O.
+Proof.
+  intros *. intro H. induction H; intros.
+  * constructor.
+  * simpl. inv H1. specialize (IHLabelStar H5 O eth Π). econstructor.
+    2: exact IHLabelStar.
+    clear H5 H0 IHLabelStar. destruct_or! H4; subst.
+    - constructor; auto.
+    - constructor; auto.
+    - constructor; auto.
+Qed.
 
-Section map_pmap.
+(* Lemma meta_to_cons_mk_list :
+  forall l l',
+    meta_to_cons l = l' <-> mk_list l' = Some l.
+Proof.
+  split; revert l'; induction l; intros; simpl in H; subst.
+  * by simpl.
+  * simpl. 
+Qed. *)
+
+Lemma meta_to_cons_mk_list : forall l, mk_list (meta_to_cons l) = Some l.
+Proof.
+  induction l.
+  by simpl.
+  simpl. by rewrite IHl.
+Qed.
+
+Lemma mk_list_meta_to_cons : forall l l', mk_list l = Some l' ->
+  meta_to_cons l' = l.
+Proof.
+  induction l; intros; inv H.
+  * by simpl.
+  * case_match. 2: congruence.
+    inv H1. simpl. f_equal.
+    by apply IHl2.
+Qed.
+
+Lemma eval_split_correct :
+  forall l l' idx,
+  mk_list l = Some l' ->
+  idx < length l' ->
+  eval_split (VLit (Z.of_nat idx)) l = RValSeq [VTuple [meta_to_cons (take idx l'); meta_to_cons (drop idx l')]].
+Proof.
+  intros. simpl.
+  case_match.
+  * apply Z.ltb_lt in H1. lia.
+  * rewrite Nat2Z.id.
+    clear H1. revert l l' H0 H. induction idx; intros.
+    - simpl. rewrite drop_0. by erewrite mk_list_meta_to_cons.
+    - simpl. destruct l; inv H. simpl in H0. lia.
+      case_match. 2: congruence. inv H2. simpl in H0.
+      specialize (IHidx l2 l ltac:(lia) H). case_match. 2: congruence.
+      destruct p. simpl.
+      by inv IHidx.
+Qed.
+
+Lemma mk_list_closed :
+  forall l l' Γ,
+    VAL Γ ⊢ l ->
+    mk_list l = Some l' -> Forall (ValScoped Γ) l'.
+Proof.
+  induction l; intros; inv H0. by constructor.
+  case_match; try congruence.
+  inv H2. constructor. by inv H.
+  apply IHl2; by destruct_scopes.
+Qed.
+
+Lemma meta_to_cons_closed :
+  forall l Γ,
+    Forall (ValScoped Γ) l ->
+    VAL Γ ⊢ meta_to_cons l.
+Proof.
+  induction l; intros; inv H; simpl; by scope_solver.
+Qed.
+
+Lemma EReceive_scope :
+  forall l time r Γ,
+  Forall (fun '(pl, g, e) => EXP PatListScope pl + (3 + Γ) ⊢ g /\ EXP PatListScope pl + (3 + Γ) ⊢ e) l ->
+  EXP 3 + Γ ⊢ time ->
+  EXP 4 + Γ ⊢ r ->
+  EXP Γ ⊢ EReceive l time r.
+Proof.
+  intros. do 6 scope_solver_step.
+  1: scope_solver.
+  2: lia.
+  do 2 scope_solver_step. scope_solver.
+  1: scope_solver.
+  do 2 scope_solver_step.
+  1: scope_solver.
+  do 2 scope_solver_step.
+  scope_solver_step.
+  1: scope_solver.
+  all: intros; simpl in *; rewrite app_length, map_length in H2; simpl in H2;
+  assert (i < length l \/ i = length l) by lia; destruct H3.
+  {
+    rewrite indexed_to_forall with (def := ([], ˝VNil, ˝VNil)) in H.
+    apply H in H3 as H'.
+    repeat rewrite map_app. repeat rewrite map_map. simpl.
+    rewrite app_nth1. 2: by rewrite map_length.
+    rewrite app_nth1. 2: by rewrite map_length.
+    rewrite map_nth with (d := ([], ˝VNil, ˝VNil)).
+    setoid_rewrite map_nth with (d := ([], ˝VNil, ˝VNil)).
+    destruct nth, p. cbn. apply H'.
+  }
+  {
+    rewrite map_nth with (d := ([], ˝VNil, ˝VNil)).
+    setoid_rewrite map_nth with (d := ([], ˝VNil, ˝VNil)).
+    subst. erewrite <- map_length. rewrite nth_middle. cbn. scope_solver.
+  }
+  {
+    rewrite indexed_to_forall with (def := ([], ˝VNil, ˝VNil)) in H.
+    apply H in H3 as H'.
+    repeat rewrite map_app. repeat rewrite map_map. simpl.
+    rewrite app_nth1. 2: by rewrite map_length.
+    rewrite app_nth1. 2: by rewrite map_length.
+    setoid_rewrite map_nth with (d := ([], ˝VNil, ˝VNil)).
+    extract_map_fun F.
+    assert (° ESeq (° EPrimOp "remove_message" []) (˝VNil) = F ([], ˝VNil, ˝VNil)). {
+      by subst F.
+    }
+    erewrite (nth_indep (map F l) _ (° ESeq (° EPrimOp "remove_message" []) (˝ VNil))).
+    rewrite H4. rewrite map_nth. subst F.
+    destruct nth, p. cbn.
+    do 2 scope_solver_step.
+    1: scope_solver.
+    1: apply H'.
+    by rewrite map_length.
+  }
+  {
+    rewrite map_nth with (d := ([], ˝VNil, ˝VNil)).
+    setoid_rewrite map_nth with (d := ([], ˝VNil, ˝VNil)).
+    subst. erewrite <- map_length. rewrite nth_middle. cbn. scope_solver.
+  }
+Qed.
+
+Lemma eval_append_correct :
+  forall l l',
+    eval_append (meta_to_cons l) (meta_to_cons l') = RValSeq [meta_to_cons (l ++ l')].
+Proof.
+  induction l; simpl; intros.
+  * reflexivity.
+  * by rewrite IHl.
+Qed.
+
+Section seq_map_eval.
 
 Context {l : Val}
         {l' : list Val}
-        {i : nat}
+        {ident : nat}
         {f : Val -> Val}
         {f_clos : Val}
-        {f_clos_closed : VALCLOSED f_clos}
-        {ι : PID} (* This PID will be observed *).
+        {f_clos_closed : VALCLOSED f_clos}.
 
 Hypothesis f_simulates :
   forall v : Val, create_result (IApp f_clos) [v] [] = Some (RValSeq [f v], []).
@@ -43,7 +193,7 @@ Definition map_body : Exp :=
     ].
 
 Definition map_clos : Val :=
-  VClos [(i, 2, map_body)] i 2 map_body.
+  VClos [(ident, 2, map_body)] ident 2 map_body.
 
 Lemma map_clos_closed :
   VALCLOSED map_clos.
@@ -96,6 +246,93 @@ Proof.
     constructor.
 Qed.
 
+
+End seq_map_eval.
+
+Hint Resolve map_clos_closed : examples.
+
+
+
+Section map_pmap.
+
+Context {l : Val}
+        {l' : list Val}
+        {ident : nat}
+        {f : Val -> Val}
+        {f_clos : Val}
+        {f_clos_closed : VALCLOSED f_clos}
+        {ι : PID} (* This PID will be observed *).
+
+Hypothesis f_simulates :
+  forall v : Val, create_result (IApp f_clos) [v] [] = Some (RValSeq [f v], []).
+Hypothesis l_is_proper : mk_list l = Some l'.
+Hypothesis f_closed : forall v, VALCLOSED v -> VALCLOSED (f v).
+Hypothesis l_closed : VALCLOSED l.
+
+Open Scope string_scope.
+
+(* Definition map_body : Exp :=
+  ECase (˝VVar 2) [
+      ([PNil], ˝ttrue, ˝VNil);
+      ([PCons PVar PVar], ˝ttrue, °ECons (EApp (˝VVar 3) [˝VVar 0])
+                                        (EApp (˝VVar 2) [˝VVar 3;˝VVar 1])
+      )
+    ].
+
+Definition map_clos : Val :=
+  VClos [(ident, 2, map_body)] ident 2 map_body.
+
+Lemma map_clos_closed :
+  VALCLOSED map_clos.
+Proof.
+  scope_solver.
+Qed.
+
+Hint Resolve map_clos_closed : examples.
+
+Open Scope string_scope.
+
+Ltac do_step := econstructor; [constructor;auto with examples| simpl].
+
+Theorem map_clos_eval :
+  ⟨[], EApp (˝map_clos) [˝f_clos; ˝l]⟩ -->* RValSeq [meta_to_cons (map f l')].
+Proof.
+  generalize dependent l'. clear l_is_proper l'.
+  induction l; intros; simpl in *; inv l_is_proper.
+  * simpl.
+    eexists. split. repeat constructor.
+    do 7 do_step.
+    econstructor. econstructor; auto. cbn.
+    do 6 do_step.
+    constructor.
+  * case_match. 2: congruence. destruct l'; inv H0. clear IHv1.
+    inv l_closed.
+    specialize (IHv2 H4 _ eq_refl). destruct IHv2 as [clock [IHv2 IHD]].
+    eexists. split.
+    {
+      inv IHv2. inv H1. clear H4.
+      simpl. constructor. constructor; auto.
+    }
+    do 7 do_step.
+    econstructor. econstructor; auto. cbn.
+    do 2 do_step.
+    econstructor. apply eval_step_case_not_match. reflexivity.
+    do 4 do_step.
+    eapply transitive_eval.
+    rewrite <- app_nil_l at 1. apply frame_indep_nil.
+    {
+      repeat rewrite vclosed_ignores_ren; auto.
+      rewrite vclosed_ignores_sub; auto.
+      exact IHD.
+    }
+    repeat rewrite vclosed_ignores_ren; auto.
+    rewrite vclosed_ignores_sub; auto.
+    do 6 do_step.
+    econstructor. econstructor; auto. simpl. by rewrite f_simulates.
+    econstructor. constructor; auto. simpl.
+    constructor.
+Qed.
+ *)
 (*
   Alternative suggestion:
   1. Have a server with a number of PIDs that compute a map of some list and function
@@ -105,35 +342,486 @@ Qed.
 *)
 
 
+Context (idx : nat)
+        (Hidx : idx < length l').
+
 (*
 pmap(F, L) ->
-  {L1, L2} = halve(L),
+  {L1, L2} = lists:split(Idx, L),
   spawn(fun(L, Addr) -> Addr ! map(F, L), [L1, self()]),
   Mapped = map(F, L2),
   receive
     L1 -> L1 ++ L2
   end
 *)
-Definition par_map : Redex :=
-  ECase (ECall (˝VLit "lists") (˝VLit "split") [˝VLit (Z.of_nat i); ˝VVar 2])
-    [
-      ([PTuple [PVar; PVar]], ˝ttrue,
-        °ESeq 
-          (°ECall (˝erlang) (˝spawn) [
-           °EFun 2 (°ECall (˝erlang) (˝send) [˝VVar 0; °EApp (˝map_clos) [˝f_clos; ˝VVar 1]]);
-           ˝VVar 0])
-        (
-          ELet 1 (°EApp (˝map_clos) [˝f_clos; ˝VVar 1])
-             (EReceive [
+Definition receive : Exp :=
+(EReceive [
                ([PVar], ˝ttrue, 
                  °ECall (˝erlang) (˝send)
                    [
                     ˝VPid ι;
-                    °ECall (˝erlang) (˝VLit "++") [˝VVar 0; ˝VVar 1]
+                    (* NOTE: the nameless approach makes it harder to guess
+                       the variable used outside the given clauses in a receive
+                                                               |
+                                                               v
+                    *)
+                    °ECall (˝erlang) (˝VLit "++") [˝VVar 0; ˝VVar 4]
                    ])
-             ] (˝infinity) (˝VNil)) (* TODO: write a receive here! *)
+             ] (˝infinity) (˝VNil)).
+
+Definition seq_sec : Exp :=
+  ELet 1 (°EApp (˝@map_clos ident) [˝f_clos; ˝VVar 2])
+             receive.
+
+Print EReceive.
+Lemma receive_closed :
+  EXP 1 ⊢ receive.
+Proof.
+  repeat constructor; simpl. 2: lia.
+  destruct i. 2: lia.
+  simpl. intros. do 4 scope_solver_step.
+  1, 2: scope_solver.
+  1-2: destruct i; intros.
+  2, 4: destruct i; try lia.
+  all: simpl. 1-2: scope_solver.
+  all: do 3 scope_solver_step.
+  1: scope_solver.
+  1: scope_solver_step.
+  1: scope_solver.
+  all: try destruct i; intros.
+  1, 3, 5, 7: simpl. 1-3:scope_solver.
+  1: do 10 scope_solver_step.
+  all: do 8 scope_solver_step.
+  all: intros; destruct i; try destruct i; try destruct i.
+  all: do 2 scope_solver_step. lia.
+  all: intros; destruct i; try destruct i; try destruct i.
+  all: scope_solver.
+Qed.
+
+Hint Resolve receive_closed : examples.
+
+Definition send_body : Exp :=
+  (°ECall (˝erlang) (˝send) [˝VVar 0; °EApp (˝@map_clos ident) [˝f_clos; ˝VVar 1]]).
+
+Definition par_map : Redex :=
+  ECase (ECall (˝VLit "lists") (˝VLit "split") [˝VLit (Z.of_nat idx); ˝l])
+    [
+      ([PTuple [PVar; PVar]], ˝ttrue,
+        °ELet 1 (°ECall (˝erlang) (˝self) [])
+          (°ESeq 
+            (°ECall (˝erlang) (˝spawn) [
+             °EFun 2 send_body;
+             °ECons (˝VVar 0) (°ECons (˝VVar 1) (˝VNil))])
+          (
+            seq_sec
+          )
         )
       )
     ].
+
+(* Implicit assumptions with this definition:
+   - Only the child communicates, there are no other messages awaiting to
+     be processed by the parent process!!!
+   - If the equivalence is based on the empty ether, errors are rules out!!!
+*)
+
+Context (ι_base : PID)
+        (Hbase : ι_base <> ι).
+
+Opaque eval_split.
+Opaque seq_sec.
+Opaque map_clos.
+Theorem split_eval O :
+  exists l,
+    (∅, ι_base ↦ inl ([], par_map, emptyBox, ∅, false) ∥ ∅) -[l]ₙ->* 
+    (∅, ι_base ↦ inl ([FParams (ICall erlang spawn) [VClos [] 0 2 send_body] [];FSeq seq_sec.[up_subst
+                (meta_to_cons (take idx l') .: meta_to_cons (drop idx l') .: idsubst)].[
+     VPid ι_base/] ], RValSeq [VCons (VPid ι_base) (VCons (meta_to_cons (take idx l')) VNil)], emptyBox, ∅, false) ∥ ∅) with O /\
+    Forall (fun x => x.1 = τ \/ exists ι, x.1 = ASelf ι) l.
+Proof.
+  eexists. split.
+  {
+    eapply closureNodeSem_trans.
+    * apply sequential_to_node.
+      do 10 do_step.
+      econstructor 2. econstructor. reflexivity. simpl.
+      unfold eval_transform_list. simpl.
+      erewrite eval_split_correct. 2-3: eassumption.
+      do 9 do_step.
+      rewrite vclosed_ignores_sub; auto with examples.
+      rewrite vclosed_ignores_sub; auto with examples.
+      constructor.
+    * eapply n_trans. apply n_other with (ι := ι_base) (a := ASelf ι_base).
+      2: set_solver.
+      constructor.
+      apply sequential_to_node.
+      do 11 do_step.
+      rewrite vclosed_ignores_sub; auto with examples.
+      rewrite vclosed_ignores_sub; auto with examples.
+      rewrite vclosed_ignores_ren; auto with examples.
+      2: {
+        apply meta_to_cons_closed.
+        apply mk_list_closed with (Γ := 0) in l_is_proper. 2: assumption.
+        by apply Forall_take.
+      }
+      rewrite vclosed_ignores_sub; auto with examples.
+      2: {
+        apply meta_to_cons_closed.
+        apply mk_list_closed with (Γ := 0) in l_is_proper. 2: assumption.
+        by apply Forall_take.
+      }
+      do 4 do_step.
+      {
+        apply meta_to_cons_closed.
+        apply mk_list_closed with (Γ := 0) in l_is_proper. 2: assumption.
+        by apply Forall_take.
+      }
+      do 4 do_step.
+      constructor.
+  }
+  {
+    apply Forall_app. split. 2: constructor.
+    1, 3: by apply Forall_repeat; left.
+    right. by eexists.
+  }
+Qed.
+Transparent eval_split.
+Transparent seq_sec.
+
+
+Definition map_seq_send :Exp :=
+  °ECall (˝erlang) (˝send)
+       [
+        ˝VPid ι;
+        °EApp (˝@map_clos ident) [˝f_clos; ˝l]
+       ].
+
+Lemma take_helper1 :
+  VALCLOSED (meta_to_cons (take idx l')).
+Proof.
+  apply meta_to_cons_closed.
+  apply mk_list_closed with (Γ := 0) in l_is_proper. 2: assumption.
+  by apply Forall_take.
+Qed.
+
+Lemma take_helper2 :
+  VALCLOSED (meta_to_cons (map f (take idx l'))).
+Proof.
+  apply meta_to_cons_closed.
+  apply mk_list_closed with (Γ := 0) in l_is_proper. 2: assumption.
+  apply list.Forall_forall. intros. apply elem_of_map_iff in H.
+  destruct_hyps. subst.
+  apply f_closed. rewrite list.Forall_forall in l_is_proper.
+  apply l_is_proper. clear-H0.
+  pose proof subseteq_take idx l'. set_solver.
+Qed.
+
+Lemma drop_helper1 :
+  VALCLOSED (meta_to_cons (drop idx l')).
+Proof.
+  apply meta_to_cons_closed.
+  apply mk_list_closed with (Γ := 0) in l_is_proper. 2: assumption.
+  by apply Forall_drop.
+Qed.
+
+Lemma drop_helper2 :
+  VALCLOSED (meta_to_cons (map f (drop idx l'))).
+Proof.
+  apply meta_to_cons_closed.
+  apply mk_list_closed with (Γ := 0) in l_is_proper. 2: assumption.
+  apply list.Forall_forall. intros. apply elem_of_map_iff in H.
+  destruct_hyps. subst.
+  apply f_closed. rewrite list.Forall_forall in l_is_proper.
+  apply l_is_proper. clear-H0.
+  pose proof subseteq_drop idx l'. set_solver.
+Qed.
+
+Opaque receive.
+(* NOTE: coercions start to tangle up here for parsing *)
+Theorem map_pmap_bisim_empty_ether :
+  (∅, ι_base ↦ inl ([], RExp (map_seq_send), emptyBox, ∅, false) ∥ ∅) ~
+  (∅, ι_base ↦ inl ([], par_map, emptyBox, ∅, false) ∥ ∅) observing {[ι]}.
+Proof.
+  opose proof* (@map_clos_eval l l' ident f f_clos).
+  all:try assumption. destruct H as [mapₖ [Hres HD]].
+  pose proof split_eval {[ι]}. destruct H as [pmapₗ [HD2 Hₗ]].
+  eapply barbedBisim_trans.
+  eapply normalisation_τ_many_bisim.
+  2: set_solver.
+  2: {
+    apply sequential_to_node.
+    do 8 do_step.
+    eapply frame_indep_core in HD.
+    exact HD.
+  }
+  1: by apply Forall_repeat.
+  simpl.
+  eapply barbedBisim_trans.
+  2: {
+    apply barbedBisim_sym. eapply normalisation_τ_self_many_bisim.
+    3: exact HD2.
+    1: assumption.
+    set_solver.
+  }
+  constructor.
+  2,4: intros; exists source, []; eexists; simpl; split; try by constructor.
+  { (* sequential process gets a signal (which can only be a send)
+       In this case, the entire concurrent map has to be evaluated!
+     *)
+    intros. assert (ι0 = ι_base). {
+      destruct A'.
+      apply deconstruct_reduction in H. destruct_hyps.
+      put (lookup ι0 : ProcessPool -> _) on H as H'.
+      setoid_rewrite lookup_insert in H'. destruct (decide (ι0 = ι_base)).
+      assumption.
+      setoid_rewrite lookup_insert_ne in H'; auto. set_solver.
+    }
+    subst.
+    assert (a = ASend ι_base ι (SMessage (meta_to_cons (map f l')))). {
+      inv H.
+      * put (lookup ι_base : ProcessPool -> _) on H2 as P.
+        setoid_rewrite lookup_insert in P. inv P. by inv H5.
+      * unfold etherPop in H2. repeat case_match; try congruence.
+        set_solver.
+      * put (lookup ι_base : ProcessPool -> _) on H1 as P.
+        setoid_rewrite lookup_insert in P. inv P.
+        destruct_or! H6; inv H2; try inv H9; cbn in *; try congruence.
+      * put (lookup ι_base : ProcessPool -> _) on H1 as P.
+        setoid_rewrite lookup_insert in P. inv P.
+        inv H2. inv H10.
+    }
+    subst. inv H. 2: { destruct_or! H6; congruence. } clear H1.
+    put (lookup ι_base : ProcessPool -> _) on H2 as P.
+    setoid_rewrite lookup_insert in P. inv P. inv H7. 
+    (* prs = ∅ *)
+    assert (forall p, ι_base ↦ p ∥ prs = ι_base ↦ p ∥ ∅) as X. {
+      intros.
+      apply map_eq. intros. put (lookup i : ProcessPool -> _) on H2 as D.
+      destruct (decide (i = ι_base)).
+      * subst. by setoid_rewrite lookup_insert.
+      * setoid_rewrite lookup_insert_ne in D; auto.
+        by setoid_rewrite lookup_insert_ne.
+    }
+    clear H2.
+    (* To be able to use eexists, we need to pose map evaluation first! *)
+    opose proof* (@map_clos_eval (meta_to_cons (take idx l')) (take idx l') ident f f_clos) as InitEval.
+    all: try eassumption.
+    1: apply meta_to_cons_mk_list.
+    1: { apply take_helper1. }
+    opose proof* (@map_clos_eval (meta_to_cons (drop idx l')) (drop idx l') ident f f_clos) as TailEval.
+    all: try eassumption.
+    1: apply meta_to_cons_mk_list.
+    1: { apply drop_helper1. }
+    destruct InitEval as [Initₖ [InitRes InitEval]].
+    destruct TailEval as [Tailₖ [TailRes TailEval]].
+    (**)
+    do 2 eexists. split.
+    {
+      (* reductions *)
+      eapply n_trans.
+      (* spawning the new process *)
+      pose proof (infinite_is_fresh [ι; ι_base]) as HF.
+      eapply n_spawn with (ι := ι_base) (ι' := fresh [ι; ι_base]).
+      2: { clear-HF. set_solver. }
+      2: {
+        admit. (* Technical - revise fresh generation on the ether + pool! that will 
+                  also be future proof for general ethers *)
+      }
+      2: {
+        admit. (* Technical *)
+      }
+      3: {
+        constructor. reflexivity.
+      }
+      1: {
+        simpl. reflexivity.
+      }
+      1: {
+        simpl. reflexivity.
+      }
+      rewrite vclosed_ignores_sub; auto with examples.
+      rewrite vclosed_ignores_sub; auto with examples.
+      (* map is evaluated in the spawned process *)
+      eapply closureNodeSem_trans.
+      {
+        apply sequential_to_node.
+        do 8 do_step.
+        eapply frame_indep_core in InitEval.
+        exact InitEval.
+      }
+      simpl.
+      repeat rewrite (vclosed_ignores_sub map_clos); auto with examples.
+      repeat rewrite (vclosed_ignores_sub f_clos); auto with examples.
+      repeat rewrite vclosed_ignores_ren; auto.
+      2: { apply drop_helper1. }
+      (* map is sent back to the parent *)
+      eapply n_trans. eapply n_send. constructor.
+      { apply take_helper2. }
+      (* map arrives to the parent *)
+      setoid_rewrite insert_commute.
+      2: {
+        pose proof (infinite_is_fresh [ι; ι_base]).
+        set_solver.
+      }
+      eapply n_trans. apply n_arrive with (ι0 := fresh [ι; ι_base]).
+      {
+        unfold etherAdd, etherPop.
+        setoid_rewrite lookup_empty.
+        setoid_rewrite lookup_insert.
+        setoid_rewrite lookup_empty.
+        setoid_rewrite insert_insert.
+        reflexivity.
+      }
+      {
+        constructor.
+      }
+      (* parent evaluates the map *)
+      eapply closureNodeSem_trans.
+      {
+        apply sequential_to_node.
+        do 2 do_step.
+        rewrite vclosed_ignores_sub.
+        2: { apply drop_helper1. }
+        eapply frame_indep_core in TailEval.
+        eapply transitive_eval. exact TailEval.
+        simpl. do_step.
+        constructor.
+      }
+      (* parent receives the first part of the map
+        This is painful :(
+      *)
+      eapply closureNodeSem_trans.
+      {
+        eapply process_local_to_node.
+        {
+  Transparent receive.
+          unfold receive, EReceive. simpl.
+          repeat rewrite vclosed_ignores_ren; try apply drop_helper2.
+          eapply lsstep. constructor. constructor. cbn. reflexivity.
+          cbn.
+          eapply lsstep. do 2 constructor.
+          eapply lsstep. do 2 constructor.
+          1: {
+            opose proof* (EReceive_scope ([([PVar], ˝ VLit "true",
+                                  ° ECall (˝ VLit "erlang") (˝ VLit "!")
+                                      [˝ VPid ι;
+                                       ° ECall (˝ VLit "erlang") 
+                                           (˝ VLit "++")
+                                           [˝ VVar 0; ˝ meta_to_cons (map f (drop idx l'))]])]) (˝VLit "infinity"%string) (˝VNil) 0).
+            2-3: scope_solver.
+            {
+              constructor; auto. split. scope_solver.
+              do 6 scope_solver_step.
+              all: intros; destruct i; try destruct i; try destruct i.
+              1,3-5,7-9,11-12: scope_solver.
+              1: scope_solver_step; eapply loosen_scope_val; try apply drop_helper2; lia.
+              all: do 6 scope_solver_step.
+            }
+            inv H. inv H2. constructor; auto.
+            intros. simpl in *.
+            specialize (H3 0 ltac:(lia)). simpl in H3. apply H3.
+          }
+          eapply lsstep. do 2 constructor.
+          eapply lsstep. apply p_local. econstructor. congruence. reflexivity.
+          simpl.
+          eapply lsstep. apply p_local. constructor.
+          eapply lsstep. apply p_local. constructor.
+          eapply lsstep. apply p_recv_peek_message_ok. reflexivity.
+          eapply lsstep. apply p_local. constructor. reflexivity.
+          simpl.
+          eapply lsstep. apply p_local. constructor.
+          eapply lsstep. apply p_local. constructor. scope_solver.
+          eapply lsstep. apply p_local. apply eval_step_case_match. reflexivity.
+          eapply lsstep. apply p_local. constructor. scope_solver.
+          eapply lsstep. apply p_local. apply eval_step_case_true. simpl.
+          rewrite idsubst_is_id_val. simpl.
+          repeat rewrite vclosed_ignores_ren; try apply drop_helper2.
+          repeat rewrite vclosed_ignores_sub; try apply drop_helper2.
+          eapply lsstep. apply p_local. constructor.
+          eapply lsstep. apply p_local. constructor.
+          1: { apply take_helper2. }
+          eapply lsstep. apply p_local. apply eval_step_case_match. reflexivity.
+          eapply lsstep. apply p_local. constructor. scope_solver.
+          eapply lsstep. apply p_local. apply eval_step_case_true. simpl.
+          (* remove message from the mailbox *)
+          eapply lsstep. apply p_local. constructor.
+          eapply lsstep. apply p_local. constructor.
+          eapply lsstep. apply p_remove_message. by cbn.
+          eapply lsstep. apply p_local. constructor.
+          repeat rewrite vclosed_ignores_sub; try apply drop_helper2.
+          (* Reading configurations is easier from here *)
+          (* evaluate send *)
+          eapply lsstep. apply p_local. constructor.
+          eapply lsstep. apply p_local. constructor. scope_solver.
+          eapply lsstep. apply p_local. constructor.
+          eapply lsstep. apply p_local. constructor. scope_solver.
+          eapply lsstep. apply p_local. constructor.
+          eapply lsstep. apply p_local. constructor. congruence.
+          eapply lsstep. apply p_local. constructor. scope_solver.
+          eapply lsstep. apply p_local. constructor.
+          (* evaluate append *)
+          eapply lsstep. apply p_local. constructor.
+          eapply lsstep. apply p_local. constructor. scope_solver.
+          eapply lsstep. apply p_local. constructor.
+          eapply lsstep. apply p_local. constructor. scope_solver.
+          eapply lsstep. apply p_local. constructor. simpl.
+          eapply lsstep. apply p_local. constructor. congruence.
+          eapply lsstep. apply p_local. constructor.
+          1: apply take_helper2.
+          eapply lsstep. apply p_local. constructor. simpl.
+          repeat rewrite vclosed_ignores_sub; try apply drop_helper2.
+          eapply lsstep. apply p_local. constructor. apply drop_helper2.
+          eapply lsstep. apply p_local. econstructor.
+          { (* evaluate the meta-theoretical simulated append *)
+            simpl. cbn.
+            rewrite eval_append_correct.
+            rewrite <- map_app, take_drop. reflexivity.
+          }
+          apply lsrefl.
+        }
+        {
+          repeat constructor.
+        }
+      }
+      (* parent sends the result *)
+      eapply n_trans. apply n_send. constructor. assumption.
+      (* the child process should be terminated for the equivalence *)
+      setoid_rewrite insert_commute.
+      2: {
+        clear. pose proof (infinite_is_fresh [ι; ι_base]).
+        set_solver.
+      }
+      eapply n_trans. apply n_other. apply p_terminate. by clear; set_solver.
+      setoid_rewrite gset_to_gmap_empty.
+      apply n_refl.
+    }
+    { (* equivalence - we need two helpers about dead processes and ether inserts *)
+      rewrite X.
+      eapply barbedBisim_trans.
+      apply dead_process_bisim with (ι := fresh [ι;ι_base]).
+      1: clear; pose proof (infinite_is_fresh [ι; ι_base]); set_solver.
+      1: clear; pose proof (infinite_is_fresh [ι; ι_base]); set_solver.
+      simpl. (* now the pools are equal, we have to do the same for the ethers *)
+      unfold etherAdd. setoid_rewrite lookup_empty.
+      setoid_rewrite lookup_insert_ne.
+      2: clear; pose proof (infinite_is_fresh [ι; ι_base]); set_solver.
+      setoid_rewrite lookup_empty.
+      setoid_rewrite insert_commute at 2.
+      2: clear; pose proof (infinite_is_fresh [ι; ι_base]); set_solver.
+      remember (_ ↦ _ ∥ _ ↦ _ ∥ ∅) as P.
+      setoid_rewrite <- HeqP.
+      remember (insert (ι_base, ι) _ ∅) as E.
+      apply ether_empty_update_bisim.
+      clear-Hbase. set_solver.
+      simpl. subst E. left.
+      setoid_rewrite lookup_insert_ne. set_solver.
+      set_solver.
+    }
+  }
+  {
+    
+  }
+Qed.
+Transparent map_clos.
 
 End map_pmap.
